extracted_code/TestEquality.ml
@@ -5,7 +5,9 @@ let get_program f =
   let len = in_channel_length x in
   let str = really_input_string x len in
   close_in x;
-  str |> Sexp.of_string |> CrTypeIF.coq_CaracaraProgram_of_sexp
+  let p = str |> Sexp.of_string |> CrTypeIF.coq_CaracaraProgram_of_sexp in
+  Shim.print_malformed_prog p 0;
+  p
 
 (* let get_general_program f =
   let x = open_in f in
