CrDslProperties.v
@@ -7,6 +7,7 @@ From MyProject Require Import CrTransformer.
 From Stdlib Require Import PArith.BinPos.
 From Stdlib Require Import List.
 Import ListNotations.
+From Stdlib Require Import Sorting.Sorted.
 
 (* Check for duplicate identifiers in the header, state, and control lists *)
 Definition check_for_duplicate_identifiers (program : CaracaraProgram) : bool :=
@@ -18,14 +19,19 @@ Definition check_for_duplicate_identifiers (program : CaracaraProgram) : bool :=
       has_duplicates varlike_equal c
   end.
 
-From Stdlib Require Import Sorting.Sorted.
-Check Sorted.
-
 (* Compare two headers based on their uids *)
 Section VarlikeCmp.
 Context {A : Type} {CrVarLike_A : CrVarLike A}.
 Definition varlike_lt (v1 v2: A) : Prop :=
   Pos.lt (get_key v1) (get_key v2).
+Definition varlike_ltb (v1 v2: A) : bool :=
+  Pos.ltb (get_key v1) (get_key v2).
+Lemma varlike_lt_ltb_lemma :
+  forall (x y : A),
+    varlike_lt x y <-> varlike_ltb x y = true.
+Proof.
+  intros x y. unfold varlike_lt, varlike_ltb. exact (iff_sym (Pos.ltb_lt _ _)).
+Qed.
 End VarlikeCmp.
 
 (* require that a transformer ends with a matchall (make no-op or otherwise explicit) *)
@@ -78,9 +84,311 @@ Definition all_network_ctrls (net : ModuleNetwork) : list Ctrl :=
 Definition well_formed_general_program (p : GeneralCaracaraProgram) : Prop :=
   let net := get_network_from_general p in
   let headers := get_headers_from_general p in
+  let sig := get_signature_from_general p in
   wf_module_network net /\
   Coqlib.list_norepet headers /\
+  Coqlib.list_norepet sig /\
   Sorted varlike_lt headers /\
+  Sorted varlike_lt sig /\
   List.Forall well_formed_module (net_modules net) /\
   Coqlib.list_norepet (all_network_states net) /\
   Coqlib.list_norepet (all_network_ctrls net).
+
+Fixpoint Sortedb {A} (leb : A -> A -> bool) (l : list A) : bool :=
+  match l with
+  | [] => true
+  | x :: rest =>
+    match rest with
+    | [] => true
+    | y :: _ => leb x y && Sortedb leb rest
+    end
+  end.
+
+Lemma sorted_is_sorted_lemma :
+  forall T (L : list T) (lt : T -> T -> Prop) (ltb : T -> T -> bool),
+    (forall x y, lt x y <-> ltb x y = true) ->
+    Sorted lt L <-> Sortedb ltb L = true.
+Proof.
+  intros T L lt ltb H_iff.
+  induction L as [| x rest IH].
+  - split; intro; [reflexivity | constructor].
+  - destruct rest as [| y rest'].
+    + split; intro; [reflexivity | repeat constructor].
+    + simpl. rewrite Bool.andb_true_iff. split.
+      * intros Hs.
+        inversion Hs as [| ? ? Hsr Hhd]; subst.
+        inversion Hhd as [| ? ? Hvlt]; subst.
+        exact (conj (proj1 (H_iff x y) Hvlt) (proj1 IH Hsr)).
+      * intros [Hlt Hsr].
+        apply Sorted_cons.
+        -- exact (proj2 IH Hsr).
+        -- apply HdRel_cons. exact (proj2 (H_iff x y) Hlt).
+Qed.
+
+Fixpoint transformer_has_defaultb (t : Transformer) : bool :=
+  match t with
+  | [] => false
+  | [rule] => match rule with
+    | Seq (SeqCtr mp _)
+    | Par (ParCtr mp _) => match mp with
+        | [] => true
+        | _ => false
+      end
+    end
+  | _ :: rest => transformer_has_defaultb rest
+  end.
+
+Lemma transformer_has_default_prop_bool_lemma :
+  forall t,
+    transformer_has_default t <-> transformer_has_defaultb t = true.
+Proof.
+  intro t. induction t as [| rule rest IH].
+  - simpl. split; intro H; [destruct H | discriminate].
+  - destruct rest as [| rule2 rest'].
+    + destruct rule as [s | p].
+      * destruct s as [mp ops]. destruct mp as [| hd tl]; simpl;
+          split; intro H; [reflexivity | exact I | destruct H | discriminate].
+      * destruct p as [mp ops]. destruct mp as [| hd tl]; simpl;
+          split; intro H; [reflexivity | exact I | destruct H | discriminate].
+    + simpl. exact IH.
+Qed.
+
+Definition well_formed_programb (p : CaracaraProgram) : bool :=
+  match p with
+  | CaracaraProgramDef h s c t =>
+      negb (has_duplicates varlike_equal h) &&
+      negb (has_duplicates varlike_equal s) &&
+      negb (has_duplicates varlike_equal c) &&
+      Sortedb varlike_ltb h &&
+      Sortedb varlike_ltb s &&
+      Sortedb varlike_ltb c &&
+      transformer_has_defaultb t
+  end.
+
+Lemma varlike_equal_refl : forall {A} {VA : CrVarLike A} (v : A),
+  varlike_equal v v = true.
+Proof.
+  intros. unfold varlike_equal. apply Pos.eqb_eq. reflexivity.
+Qed.
+
+Lemma varlike_equal_sym_bool : forall {A} {VA : CrVarLike A} (v1 v2 : A),
+  varlike_equal v1 v2 = varlike_equal v2 v1.
+Proof.
+  intros. unfold varlike_equal.
+  destruct (Pos.eqb (get_key v1) (get_key v2)) eqn:H12;
+  destruct (Pos.eqb (get_key v2) (get_key v1)) eqn:H21;
+  try reflexivity; exfalso.
+  - apply Pos.eqb_eq in H12. rewrite H12 in H21.
+    assert (Hrefl : Pos.eqb (get_key v2) (get_key v2) = true) by (apply Pos.eqb_eq; reflexivity).
+    congruence.
+  - apply Pos.eqb_eq in H21. rewrite <- H21 in H12.
+    assert (Hrefl : Pos.eqb (get_key v1) (get_key v1) = true) by (apply Pos.eqb_eq; reflexivity).
+    congruence.
+Qed.
+
+Lemma list_norepet_implies_no_duplicates :
+  forall {A} {VA : CrVarLike A} (l : list A),
+    Coqlib.list_norepet l -> has_duplicates varlike_equal l = false.
+Proof.
+  intros A VA l Hnr.
+  induction Hnr as [| x xs Hni Hnr IH].
+  - reflexivity.
+  - simpl.
+    destruct (List.existsb (fun y => varlike_equal y x) xs) eqn:He.
+    + exfalso.
+      apply List.existsb_exists in He.
+      destruct He as [y [Hyin Heqyx]].
+      apply varlike_equal_lemma in Heqyx.
+      rewrite <- Heqyx in Hyin.
+      exact (Hni Hyin).
+    + exact IH.
+Qed.
+
+Lemma well_formed_program_prop_bool_lemma :
+  forall p,
+    well_formed_program p <-> well_formed_programb p = true.
+Proof.
+  intro p. destruct p as [h s c t].
+  unfold well_formed_program, well_formed_programb.
+  (* Instantiate sorted_is_sorted_lemma with explicit type to bypass typeclass ambiguity *)
+  pose proof (sorted_is_sorted_lemma Header h varlike_lt varlike_ltb
+    (fun x y => iff_sym (Pos.ltb_lt (get_key x) (get_key y)))) as SIFFh.
+  pose proof (sorted_is_sorted_lemma State s varlike_lt varlike_ltb
+    (fun x y => iff_sym (Pos.ltb_lt (get_key x) (get_key y)))) as SIFFs.
+  pose proof (sorted_is_sorted_lemma Ctrl c varlike_lt varlike_ltb
+    (fun x y => iff_sym (Pos.ltb_lt (get_key x) (get_key y)))) as SIFFc.
+  split.
+  - intros (Hnrh & Hnrs & Hnrc & Sorh & Sors & Sorc & Hthd).
+    pose proof (list_norepet_implies_no_duplicates h Hnrh) as Hdh.
+    pose proof (list_norepet_implies_no_duplicates s Hnrs) as Hds.
+    pose proof (list_norepet_implies_no_duplicates c Hnrc) as Hdc.
+    pose proof (proj1 SIFFh Sorh) as HSh.
+    pose proof (proj1 SIFFs Sors) as HSs.
+    pose proof (proj1 SIFFc Sorc) as HSc.
+    pose proof (proj1 (transformer_has_default_prop_bool_lemma t) Hthd) as HTt.
+    rewrite Hdh, Hds, Hdc, HSh, HSs, HSc, HTt. reflexivity.
+  - intro Hb.
+    repeat rewrite Bool.andb_true_iff in Hb.
+    destruct Hb as ((((((HnDh & HnDs) & HnDc) & HSh) & HSs) & HSc) & HTt).
+    rewrite Bool.negb_true_iff in HnDh, HnDs, HnDc.
+    repeat split.
+    + exact (has_duplicates_correct _ varlike_equal varlike_equal_refl varlike_equal_sym_bool h HnDh).
+    + exact (has_duplicates_correct _ varlike_equal varlike_equal_refl varlike_equal_sym_bool s HnDs).
+    + exact (has_duplicates_correct _ varlike_equal varlike_equal_refl varlike_equal_sym_bool c HnDc).
+    + exact (proj2 SIFFh HSh).
+    + exact (proj2 SIFFs HSs).
+    + exact (proj2 SIFFc HSc).
+    + exact (proj2 (transformer_has_default_prop_bool_lemma t) HTt).
+Qed.
+
+Definition well_formed_moduleb (m : CrModule) : bool :=
+  match m with
+  | ParserModule _ _ => true
+  | TransformerModule _ states ctrls t =>
+      negb (has_duplicates varlike_equal states) &&
+      negb (has_duplicates varlike_equal ctrls) &&
+      Sortedb varlike_ltb states &&
+      Sortedb varlike_ltb ctrls &&
+      transformer_has_defaultb t
+  end.
+
+Lemma well_formed_module_prop_bool_lemma :
+  forall m,
+    well_formed_module m <-> well_formed_moduleb m = true.
+Proof.
+  intros.
+  unfold well_formed_module, well_formed_moduleb.
+  destruct m; try (split; intros; reflexivity).
+  pose proof (sorted_is_sorted_lemma State s varlike_lt varlike_ltb
+    (fun x y => iff_sym (Pos.ltb_lt (get_key x) (get_key y)))) as SIFFs.
+  pose proof (sorted_is_sorted_lemma Ctrl c varlike_lt varlike_ltb
+    (fun x y => iff_sym (Pos.ltb_lt (get_key x) (get_key y)))) as SIFFc.
+  split; intros.
+  - destruct H as (Hnrs & Hnrc & HSs & HSc & HTd).
+    apply list_norepet_implies_no_duplicates in Hnrs.
+    apply list_norepet_implies_no_duplicates in Hnrc.
+    apply (proj1 SIFFs) in HSs.
+    apply (proj1 SIFFc) in HSc.
+    apply transformer_has_default_prop_bool_lemma in HTd.
+    rewrite Hnrs, Hnrc, HSs, HSc, HTd. reflexivity.
+  - repeat rewrite Bool.andb_true_iff in H.
+    destruct H as ((((HnDs & HnDc) & HSs) & HSc) & HTd).
+    rewrite Bool.negb_true_iff in HnDs, HnDc.
+    repeat split.
+    + exact (has_duplicates_correct _ varlike_equal varlike_equal_refl
+               varlike_equal_sym_bool s HnDs).
+    + exact (has_duplicates_correct _ varlike_equal varlike_equal_refl
+               varlike_equal_sym_bool c HnDc).
+    + exact (proj2 SIFFs HSs).
+    + exact (proj2 SIFFc HSc).
+    + apply transformer_has_default_prop_bool_lemma. exact HTd.
+Qed.
+
+Definition well_formed_general_programb (p : GeneralCaracaraProgram) : bool :=
+  let net := get_network_from_general p in
+  let headers := get_headers_from_general p in
+  let sig := get_signature_from_general p in
+  wf_module_networkb net &&
+  negb (has_duplicates varlike_equal headers) &&
+  negb (has_duplicates varlike_equal sig) &&
+  Sortedb varlike_ltb headers &&
+  Sortedb varlike_ltb sig &&
+  List.forallb well_formed_moduleb (net_modules net) &&
+  negb (has_duplicates varlike_equal (all_network_states net)) &&
+  negb (has_duplicates varlike_equal (all_network_ctrls net)).
+
+Lemma well_formed_general_program_prop_bool_lemma :
+  forall p,
+    well_formed_general_program p <-> well_formed_general_programb p = true.
+Proof.
+  intros p.
+  destruct p as [headers net sig].
+  unfold well_formed_general_program, well_formed_general_programb.
+  simpl.
+  pose proof (sorted_is_sorted_lemma Header headers varlike_lt varlike_ltb
+    (fun x y => iff_sym (Pos.ltb_lt (get_key x) (get_key y)))) as SIFFh.
+  pose proof (sorted_is_sorted_lemma Header sig varlike_lt varlike_ltb
+    (fun x y => iff_sym (Pos.ltb_lt (get_key x) (get_key y)))) as SIFFsig.
+
+  (* Reflection of [List.Forall] against [List.forallb] for well-formed
+     modules. *)
+  assert (FAFB : List.Forall well_formed_module (net_modules net) <->
+                 List.forallb well_formed_moduleb (net_modules net) = true).
+  { rewrite Forall_forall, forallb_forall. split; intros H x Hx;
+      apply well_formed_module_prop_bool_lemma; auto. }
+
+  (* Reflexivity, symmetry, and injectivity of [posesque_eqb] on
+     [ModuleName].  Used to handle [mod_names_unique{,b}] below. *)
+  assert (Hpr : forall x : ModuleName, posesque_eqb x x = true).
+  { intros [q]. unfold posesque_eqb. simpl. apply Pos.eqb_refl. }
+  assert (Hps : forall x y : ModuleName, posesque_eqb x y = posesque_eqb y x).
+  { intros [q1] [q2]. unfold posesque_eqb. simpl.
+    destruct (Pos.eqb q1 q2) eqn:E12, (Pos.eqb q2 q1) eqn:E21;
+      try reflexivity; exfalso.
+    - apply Pos.eqb_eq in E12. subst. rewrite Pos.eqb_refl in E21. discriminate.
+    - apply Pos.eqb_eq in E21. subst. rewrite Pos.eqb_refl in E12. discriminate. }
+  assert (Hpeq : forall x y : ModuleName, posesque_eqb x y = true -> x = y).
+  { intros [q1] [q2] H. unfold posesque_eqb in H. simpl in H.
+    apply Pos.eqb_eq in H. f_equal; exact H. }
+
+  (* [mod_names_unique <-> mod_names_uniqueb = true]. *)
+  assert (MNU : mod_names_unique net <-> mod_names_uniqueb net = true).
+  { unfold mod_names_unique, mod_names_uniqueb. split.
+    - intros Hnr. apply Bool.negb_true_iff.
+      induction Hnr as [| x xs Hni _ IH].
+      + reflexivity.
+      + simpl.
+        destruct (List.existsb (fun y => posesque_eqb y x) xs) eqn:He.
+        * exfalso. apply List.existsb_exists in He.
+          destruct He as [y [Hyin Heqyx]]. apply Hpeq in Heqyx.
+          subst. exact (Hni Hyin).
+        * exact IH.
+    - intros Hb. apply Bool.negb_true_iff in Hb.
+      exact (has_duplicates_correct _ posesque_eqb Hpr Hps _ Hb). }
+
+  (* [wf_module_network <-> wf_module_networkb = true]. *)
+  assert (WFB : wf_module_network net <-> wf_module_networkb net = true).
+  { unfold wf_module_network, wf_module_networkb.
+    pose proof (start_module_defined_prop_bool_lemma net) as SMD.
+    pose proof (is_dag_prop_bool_lemma net) as IDP.
+    split.
+    - intros (HMU & HSM & HDG).
+      rewrite (proj1 MNU HMU), (proj1 SMD HSM), (proj1 IDP HDG).
+      reflexivity.
+    - intros Hb. repeat rewrite Bool.andb_true_iff in Hb.
+      destruct Hb as ((HMU & HSM) & HDG).
+      split; [apply MNU | split; [apply SMD | apply IDP]]; assumption. }
+
+  split.
+  - intros (Hwf & Hnrh & Hnrsig & HSh & HSsig & HFa & Hnrst & Hnrct).
+    apply WFB in Hwf.
+    apply list_norepet_implies_no_duplicates in Hnrh.
+    apply list_norepet_implies_no_duplicates in Hnrsig.
+    apply (proj1 SIFFh) in HSh.
+    apply (proj1 SIFFsig) in HSsig.
+    apply FAFB in HFa.
+    apply list_norepet_implies_no_duplicates in Hnrst.
+    apply list_norepet_implies_no_duplicates in Hnrct.
+    rewrite Hwf, Hnrh, Hnrsig, HSh, HSsig, HFa, Hnrst, Hnrct.
+    reflexivity.
+  - intros Hb.
+    repeat rewrite Bool.andb_true_iff in Hb.
+    destruct Hb as (((((((Hwf & Hnrh) & Hnrsig) & HSh) & HSsig) & HFa) & Hnrst)
+                    & Hnrct).
+    rewrite Bool.negb_true_iff in Hnrh, Hnrsig, Hnrst, Hnrct.
+    (* Build the 8-way conjunction explicitly with [conj] so the
+       transparent [wf_module_network] is not unfolded by [split]. *)
+    refine (conj _ (conj _ (conj _ (conj _ (conj _ (conj _ (conj _ _))))))).
+    + apply (proj2 WFB). exact Hwf.
+    + exact (has_duplicates_correct _ varlike_equal varlike_equal_refl
+               varlike_equal_sym_bool headers Hnrh).
+    + exact (has_duplicates_correct _ varlike_equal varlike_equal_refl
+               varlike_equal_sym_bool sig Hnrsig).
+    + exact (proj2 SIFFh HSh).
+    + exact (proj2 SIFFsig HSsig).
+    + apply (proj2 FAFB). exact HFa.
+    + exact (has_duplicates_correct _ varlike_equal varlike_equal_refl
+               varlike_equal_sym_bool (all_network_states net) Hnrst).
+    + exact (has_duplicates_correct _ varlike_equal varlike_equal_refl
+               varlike_equal_sym_bool (all_network_ctrls net) Hnrct).
+Qed.
