CrIdentifiers.v
@@ -10,45 +10,101 @@ Inductive Header : Type := HeaderCtr (uid : positive).
 Inductive State : Type := StateCtr (uid : positive).
 Inductive ModuleName : Type := ModuleNameCtr (uid : positive).
 Inductive FunctionName : Type := FunctionNameCtr (uid : positive).
-Inductive ConnectionName : Type := ConnectionNameCtr (uid : positive).
 Inductive Ctrl : Type := CtrlCtr (uid : positive).
 
-(* Equality check functions for the identifiers above *)
-Definition parser_state_equal (p1 p2 : ParserState) :=
-    match p1, p2 with
-            | ParserStateCtr xid, ParserStateCtr yid => Pos.eqb xid yid
-    end.
+Class Posesque (A : Type) := {
+  wrap       : positive -> A;
+  unwrap     : A -> positive;
+  incr       : A -> A;
+  unwrap_inj : forall x y : A, unwrap x = unwrap y -> x = y;
+}.
 
-Definition module_name_equal (m1 m2 : ModuleName) :=
-    match m1, m2 with
-            | ModuleNameCtr xid, ModuleNameCtr yid => Pos.eqb xid yid
-    end.
+Instance Posesque_ParserState : Posesque ParserState := {
+  wrap := fun p => ParserStateCtr p;
+  unwrap := fun s => match s with ParserStateCtr p => p end;
+  incr := fun s => match s with ParserStateCtr p => ParserStateCtr (p + 1) end;
+  unwrap_inj :=
+    fun x y => match x, y with
+               | ParserStateCtr px, ParserStateCtr py =>
+                   fun H => f_equal ParserStateCtr H
+               end;
+}.
+Instance Posesque_Header : Posesque Header := {
+  wrap := fun p => HeaderCtr p;
+  unwrap := fun s => match s with HeaderCtr p => p end;
+  incr := fun s => match s with HeaderCtr p => HeaderCtr (p + 1) end;
+  unwrap_inj :=
+    fun x y => match x, y with
+               | HeaderCtr px, HeaderCtr py =>
+                   fun H => f_equal HeaderCtr H
+               end;
+}.
+Instance Posesque_State : Posesque State := {
+  wrap := fun p => StateCtr p;
+  unwrap := fun s => match s with StateCtr p => p end;
+  incr := fun s => match s with StateCtr p => StateCtr (p + 1) end;
+  unwrap_inj :=
+    fun x y => match x, y with
+               | StateCtr px, StateCtr py =>
+                   fun H => f_equal StateCtr H
+               end;
+}.
+Instance Posesque_ModuleName : Posesque ModuleName := {
+  wrap := fun p => ModuleNameCtr p;
+  unwrap := fun s => match s with ModuleNameCtr p => p end;
+  incr := fun s => match s with ModuleNameCtr p => ModuleNameCtr (p + 1) end;
+  unwrap_inj :=
+    fun x y => match x, y with
+               | ModuleNameCtr px, ModuleNameCtr py =>
+                   fun H => f_equal ModuleNameCtr H
+               end;
+}.
+Instance Posesque_FunctionName : Posesque FunctionName := {
+  wrap := fun p => FunctionNameCtr p;
+  unwrap := fun s => match s with FunctionNameCtr p => p end;
+  incr := fun s => match s with FunctionNameCtr p => FunctionNameCtr (p + 1) end;
+  unwrap_inj :=
+    fun x y => match x, y with
+               | FunctionNameCtr px, FunctionNameCtr py =>
+                   fun H => f_equal FunctionNameCtr H
+               end;
+}.
+Instance Posesque_Ctrl : Posesque Ctrl := {
+  wrap := fun p => CtrlCtr p;
+  unwrap := fun s => match s with CtrlCtr p => p end;
+  incr := fun s => match s with CtrlCtr p => CtrlCtr (p + 1) end;
+  unwrap_inj :=
+    fun x y => match x, y with
+               | CtrlCtr px, CtrlCtr py =>
+                   fun H => f_equal CtrlCtr H
+               end;
+}.
 
-Definition function_name_equal (f1 f2 : FunctionName) :=
-    match f1, f2 with
-            | FunctionNameCtr xid, FunctionNameCtr yid => Pos.eqb xid yid
-    end.
-
-Definition connection_name_equal (c1 c2 : ConnectionName) :=
-    match c1, c2 with
-            | ConnectionNameCtr xid, ConnectionNameCtr yid => Pos.eqb xid yid
-    end.
-
-(* Decidable equality for the varlike identifiers, derived from positive equality. *)
-Definition header_eq_dec : forall x y : Header, {x = y} + {x <> y}.
+Section Posesque.
+Context {A : Type} {asdf : Posesque A}.
+Definition posesque_eq (v1 v2: A) : Prop :=
+  Pos.eq (unwrap v1) (unwrap v2).
+Definition posesque_eqb (v1 v2: A) : bool :=
+  Pos.eqb (unwrap v1) (unwrap v2).
+Lemma posesque_eq_eqb :
+  forall v1 v2,
+    posesque_eq v1 v2 <-> posesque_eqb v1 v2 = true.
 Proof.
-  intros [a] [b]. destruct (Pos.eq_dec a b);
-    [left; subst; reflexivity | right; intro Heq; inversion Heq; contradiction].
-Defined.
-
-Definition state_eq_dec : forall x y : State, {x = y} + {x <> y}.
+  intros. unfold posesque_eq, posesque_eqb.
+  rewrite Pos.eqb_eq. reflexivity.
+Qed.
+Lemma posesque_eqb_iff :
+  forall (x y : A), posesque_eqb x y = true <-> x = y.
 Proof.
-  intros [a] [b]. destruct (Pos.eq_dec a b);
-    [left; subst; reflexivity | right; intro Heq; inversion Heq; contradiction].
-Defined.
-
-Definition ctrl_eq_dec : forall x y : Ctrl, {x = y} + {x <> y}.
+  intros. unfold posesque_eqb. split.
+  - intros H. apply Pos.eqb_eq in H. apply unwrap_inj. exact H.
+  - intros H. inversion H. apply Pos.eqb_refl.
+Qed.
+Definition posesque_eq_dec (x y : A) : {x = y} + {x <> y}.
 Proof.
-  intros [a] [b]. destruct (Pos.eq_dec a b);
-    [left; subst; reflexivity | right; intro Heq; inversion Heq; contradiction].
+  destruct (posesque_eqb x y) eqn:Heq.
+  - left. apply posesque_eqb_iff. exact Heq.
+  - right. intros H. apply posesque_eqb_iff in H.
+    rewrite H in Heq. discriminate.
 Defined.
+End Posesque.
