Extraction.v
@@ -10,6 +10,7 @@ From MyProject Require Import TestPrograms.
 From MyProject Require Import TestModulePrograms.
 From MyProject Require Import PktClass.
 From MyProject Require Import CrTModConcreteSemantics.
+From MyProject Require Import CrDslProperties.
 
 (* Tell extraction to use your external OCaml implementation *)
 Extract Constant smt_query => "Z3Solver.solve".
@@ -25,8 +26,8 @@ Separate Extraction
   CrSymbolicSemanticsTransformer.eval_sym_state
   CrConcreteSemanticsTransformer.eval_cr_program_concrete
   CrVarLike.program_state_mapper CrVarLike.init_concrete_state
-  test_programs
-  mod_test_programs
+  test_programs mod_test_programs
   CrVarLike.init_general_concrete_state
   CrTModConcreteSemantics.eval_general_program_concrete_sinks
-  PktClass.ex_lin_prog PktClass.ex_tss_prog modnet_equivalence_checker.
+  PktClass.ex_lin_prog PktClass.ex_tss_prog modnet_equivalence_checker
+  well_formed_programb well_formed_general_programb.
