PosGraphLemmas.v
@@ -1,0 +1,377 @@
+From Stdlib Require Import List.
+From Stdlib Require Import Arith.
+From Stdlib Require Import Lia.
+Import ListNotations.
+From MyProject Require Import CrIdentifiers.
+From MyProject Require Import Coqlib.
+From MyProject Require Import ListUtils.
+From Stdlib Require Import PArith.BinPos.
+
+
+Local Open Scope list_scope.
+Local Open Scope nat_scope.
+
+Section PosGraph.
+Context {A : Type} {PA : Posesque A}.
+
+Definition graph := A -> A -> bool.
+
+Fixpoint is_walk (g : graph) (vs : list A) : Prop :=
+  match vs with
+  | [] => False
+  | [_] => True
+  | u :: (v :: _) as rest => g u v = true /\ is_walk g rest
+  end.
+
+Definition reaches (g : graph) (x y : A) : Prop :=
+  exists mid : list A,
+    is_walk g (x :: mid ++ [y]).
+
+Fixpoint reachableb (g : graph) (nodes : list A) (fuel : nat)
+                     (src dst : A) : bool :=
+  match fuel with
+  | O => g src dst
+  | S fuel' =>
+      g src dst
+      || existsb (fun w => g src w && reachableb g nodes fuel' w dst) nodes
+  end.
+
+Definition is_dag (g : graph) : Prop :=
+  forall x : A, ~ reaches g x x.
+
+Definition is_dagb (g : graph) (nodes : list A) : bool :=
+  forallb (fun x => negb (reachableb g nodes (length nodes) x x)) nodes.
+
+(* ------------------------------------------------------------------ *)
+(* Helper: edges stay inside [nodes].                                 *)
+(* ------------------------------------------------------------------ *)
+
+Definition Aeqb (x y : A) : bool := posesque_eqb x y.
+
+Lemma Aeqb_true_iff : forall x y, Aeqb x y = true <-> x = y.
+Proof. intros. apply posesque_eqb_iff. Qed.
+
+Lemma Aeqb_refl : forall x, Aeqb x x = true.
+Proof. intros. apply Aeqb_true_iff. reflexivity. Qed.
+
+Definition Aeq_dec (x y : A) : {x = y} + {x <> y} := posesque_eq_dec x y.
+
+(* ------------------------------------------------------------------ *)
+(* Relating walks to bounded reachability                             *)
+(* ------------------------------------------------------------------ *)
+
+Lemma reachableb_sound :
+  forall g nodes fuel src dst,
+    reachableb g nodes fuel src dst = true ->
+    reaches g src dst.
+Proof.
+  intros g nodes fuel.
+  induction fuel as [|fuel' IH]; intros src dst H.
+  - (* fuel = 0 : direct edge *)
+    simpl in H. exists []. simpl. split; [exact H | exact I].
+  - simpl in H. apply orb_prop in H. destruct H as [H | H].
+    + (* direct edge *)
+      exists []. simpl. split; [exact H | exact I].
+    + apply existsb_exists in H. destruct H as [w [_ Hw]].
+      apply andb_prop in Hw. destruct Hw as [Hedge Hrec].
+      apply IH in Hrec. destruct Hrec as [mid Hwalk].
+      (* edge src -> w, then walk w ... dst *)
+      exists (w :: mid).
+      simpl. split.
+      * exact Hedge.
+      * exact Hwalk.
+Qed.
+
+Lemma walk_reachableb :
+  forall g nodes mid src dst,
+    (forall w, In w mid -> In w nodes) ->
+    is_walk g (src :: mid ++ [dst]) ->
+    length mid <= length nodes ->
+    reachableb g nodes (length nodes) src dst = true.
+Proof.
+  assert (gen :
+    forall g nodes mid src dst fuel,
+      (forall w, In w mid -> In w nodes) ->
+      is_walk g (src :: mid ++ [dst]) ->
+      length mid <= fuel ->
+      reachableb g nodes fuel src dst = true).
+  { intros g nodes mid. induction mid as [|m mid' IH];
+      intros src dst fuel Hin Hwalk Hlen.
+    - (* mid = [] : single edge src -> dst *)
+      simpl in Hwalk. destruct Hwalk as [Hedge _].
+      destruct fuel; simpl.
+      + exact Hedge.
+      + rewrite Hedge. reflexivity.
+    - (* mid = m :: mid' *)
+      simpl in Hwalk. destruct Hwalk as [Hedge Hrest].
+      destruct fuel as [|fuel'].
+      + simpl in Hlen. lia.
+      + simpl. apply orb_true_intro. right.
+        apply existsb_exists. exists m. split.
+        * apply Hin. left. reflexivity.
+        * apply andb_true_intro. split.
+          -- exact Hedge.
+          -- apply IH.
+             ++ intros w Hw. apply Hin. right. exact Hw.
+             ++ exact Hrest.
+             ++ simpl in Hlen. lia. }
+  intros g nodes mid src dst Hin Hwalk Hlen.
+  eapply gen; eauto.
+Qed.
+
+(* ------------------------------------------------------------------ *)
+(* Shortening walks: a walk whose intermediate vertices all lie in     *)
+(* [nodes] can be reduced to one with no repeated intermediate vertex, *)
+(* hence with at most |nodes| intermediate vertices.                   *)
+(* ------------------------------------------------------------------ *)
+
+Lemma is_walk_app :
+  forall g a l1 w l2,
+    is_walk g (a :: l1 ++ [w]) ->
+    is_walk g (w :: l2) ->
+    is_walk g (a :: l1 ++ w :: l2).
+Proof.
+  intros g a l1. revert a.
+  induction l1 as [|b l1' IH]; intros a w l2 H1 H2.
+  - (* l1 = [] : walk is a :: [w], second is w :: l2 *)
+    simpl in H1. destruct H1 as [Hedge _].
+    simpl. destruct l2 as [|c l2'].
+    + simpl. split; [exact Hedge | exact I].
+    + simpl. split; [exact Hedge | exact H2].
+  - (* l1 = b :: l1' *)
+    simpl in H1. destruct H1 as [Hedge Hrest].
+    simpl. split.
+    + exact Hedge.
+    + change (is_walk g (b :: l1' ++ w :: l2)).
+      apply IH.
+      * exact Hrest.
+      * exact H2.
+Qed.
+
+Lemma walk_mid_in_nodes :
+  forall g nodes x mid y,
+    (forall u v, g u v = true -> In u nodes /\ In v nodes) ->
+    is_walk g (x :: mid ++ [y]) ->
+    forall w, In w mid -> In w nodes.
+Proof.
+  intros g nodes x mid. revert x.
+  induction mid as [|m mid' IH]; intros x y Hedges Hwalk w Hw.
+  - simpl in Hw. contradiction.
+  - simpl in Hwalk. destruct Hwalk as [Hedge Hrest].
+    simpl in Hw. destruct Hw as [Heq | Hw].
+    + subst w. apply (Hedges x m Hedge).
+    + eapply IH; eauto.
+Qed.
+
+(* ------------------------------------------------------------------ *)
+(* Pigeonhole: a reaches-walk can be made short.                       *)
+(* ------------------------------------------------------------------ *)
+
+Lemma remove_one_repeat :
+  forall g x y mid,
+    is_walk g (x :: mid ++ [y]) ->
+    has_duplicates Aeqb mid = true ->
+    exists mid',
+      is_walk g (x :: mid' ++ [y]) /\ length mid' < length mid.
+Proof.
+  intros g x y mid Hwalk Hdup.
+  (* Find a duplicated element and split. *)
+  (* From has_duplicates = true, get w appearing twice. *)
+  assert (exists (l1 : list A) (w : A) (l2 l3 : list A),
+            mid = l1 ++ w :: l2 ++ w :: l3) as Hsplit.
+  { clear Hwalk. induction mid as [|a mid' IH].
+    - simpl in Hdup. discriminate.
+    - simpl in Hdup.
+      destruct (existsb (fun y0 => Aeqb y0 a) mid') eqn:Hex.
+      + apply existsb_exists in Hex. destruct Hex as [b [Hbin Hbeq]].
+        apply Aeqb_true_iff in Hbeq. subst b.
+        apply in_split in Hbin. destruct Hbin as [l2 [l3 Hmid']].
+        exists [], a, l2, l3. simpl. rewrite Hmid'. reflexivity.
+      + apply IH in Hdup. destruct Hdup as [l1 [w [l2 [l3 Heq]]]].
+        exists (a :: l1), w, l2, l3. simpl. rewrite Heq. reflexivity. }
+  destruct Hsplit as [l1 [w [l2 [l3 Hmid]]]].
+  subst mid.
+  (* The walk is x :: l1 ++ w :: l2 ++ w :: l3 ++ [y].
+     Cut out the segment between the two w's:
+     new walk: x :: l1 ++ w :: l3 ++ [y]. *)
+  exists (l1 ++ w :: l3).
+  split.
+  - (* build the shortened walk *)
+    (* original: is_walk g (x :: (l1 ++ w :: l2 ++ w :: l3) ++ [y]) *)
+    (* We will split the original into prefix walk to w and suffix walk
+       from the second w. *)
+    (* Use is_walk_app with a:=x, l1 := l1 ++ [w], l2 := l3 ++ [y]. *)
+    (* First, extract that the prefix x :: l1 ++ [w] is a walk, and that
+       w :: l3 ++ [y] is a walk. *)
+    assert (Hpre : is_walk g (x :: l1 ++ [w])).
+    { (* prefix of the original walk *)
+      revert Hwalk. clear.
+      generalize (l2 ++ w :: l3 ++ [y]).
+      intro tail. revert x.
+      induction l1 as [|a l1' IH]; intros x Hwalk.
+      - simpl. simpl in Hwalk. destruct Hwalk as [Hedge _].
+        split; [exact Hedge | exact I].
+      - simpl in Hwalk. destruct Hwalk as [Hedge Hrest].
+        simpl. split.
+        + exact Hedge.
+        + change (is_walk g (a :: l1' ++ [w])).
+          apply IH. exact Hrest. }
+    assert (Hsuf : is_walk g (w :: l3 ++ [y])).
+    { (* suffix of the original walk: skip x :: l1 ++ [w] ++ l2 *)
+      revert Hwalk. clear.
+      (* The original tail after the first w is: w :: l2 ++ w :: l3 ++ [y].
+         We need a walk from the SECOND w.  First obtain the walk starting
+         at the first w, then peel l2 to reach the second w. *)
+      (* Get walk starting at first w. *)
+      assert (Hstart :
+        forall pre z,
+          is_walk g (z :: pre ++ (w :: l2 ++ w :: l3 ++ [y])) ->
+          is_walk g (w :: l2 ++ w :: l3 ++ [y])).
+      { induction pre as [|a pre' IH]; intros z Hw.
+        - simpl in Hw. destruct Hw as [_ Hrest]. exact Hrest.
+        - apply (IH a).
+          change (is_walk g (z :: a :: pre' ++ w :: l2 ++ w :: l3 ++ [y]))
+            in Hw.
+          destruct Hw as [_ Hrest]. exact Hrest. }
+      intro Hwalk.
+      assert (Hwfull : is_walk g (w :: l2 ++ w :: l3 ++ [y])).
+      { apply (Hstart l1 x).
+        (* Hwalk : is_walk g (x :: (l1 ++ w :: l2 ++ w :: l3) ++ [y]) *)
+        replace (l1 ++ w :: l2 ++ w :: l3 ++ [y])
+           with ((l1 ++ w :: l2 ++ w :: l3) ++ [y]).
+        2:{ rewrite <- app_assoc. simpl.
+            rewrite <- app_assoc. simpl. reflexivity. }
+        exact Hwalk. }
+      (* Now peel l2 from w :: l2 ++ w :: ... to reach the second w. *)
+      revert Hwfull. clear.
+      assert (Hpeel :
+        forall pre z,
+          is_walk g (z :: pre ++ (w :: l3 ++ [y])) ->
+          is_walk g (w :: l3 ++ [y])).
+      { induction pre as [|a pre' IH]; intros z Hw.
+        - simpl in Hw. destruct Hw as [_ Hrest]. exact Hrest.
+        - apply (IH a).
+          change (is_walk g (z :: a :: pre' ++ w :: l3 ++ [y])) in Hw.
+          destruct Hw as [_ Hrest]. exact Hrest. }
+      intro Hwfull. apply (Hpeel l2 w). exact Hwfull. }
+    (* combine prefix (x..w) and suffix (w..y) *)
+    replace (x :: (l1 ++ w :: l3) ++ [y])
+       with (x :: l1 ++ w :: (l3 ++ [y])).
+    2:{ rewrite <- app_assoc. simpl. reflexivity. }
+    apply is_walk_app.
+    + exact Hpre.
+    + exact Hsuf.
+  - (* length decreases: we removed [w] ++ l2 (at least one element) *)
+    repeat rewrite length_app. simpl.
+    repeat rewrite length_app. simpl. lia.
+Qed.
+
+Lemma shorten_walk_nodup :
+  forall g x y mid,
+    is_walk g (x :: mid ++ [y]) ->
+    exists mid',
+      is_walk g (x :: mid' ++ [y]) /\
+      has_duplicates Aeqb mid' = false /\
+      length mid' <= length mid.
+Proof.
+  intros g x y mid.
+  remember (length mid) as n eqn:Hn.
+  revert mid Hn.
+  induction n as [n IH] using (well_founded_induction lt_wf);
+    intros mid Hn Hwalk.
+  destruct (has_duplicates Aeqb mid) eqn:Hdup.
+  - destruct (remove_one_repeat g x y mid Hwalk Hdup)
+      as [mid' [Hwalk' Hlen]].
+    destruct (IH (length mid') ltac:(lia) mid' eq_refl Hwalk')
+      as [mid'' [Hw'' [Hd'' Hl'']]].
+    exists mid''. split; [exact Hw'' | split; [exact Hd'' | lia]].
+  - exists mid. split; [exact Hwalk | split; [exact Hdup | lia]].
+Qed.
+
+Lemma Aeqb_sym : forall a b, Aeqb a b = Aeqb b a.
+Proof.
+  intros a b. unfold Aeqb, posesque_eqb.
+  destruct (Pos.eqb (unwrap a) (unwrap b)) eqn:E.
+  - symmetry. apply Pos.eqb_eq. apply Pos.eqb_eq in E. auto.
+  - symmetry. apply Pos.eqb_neq. apply Pos.eqb_neq in E. auto.
+Qed.
+
+Lemma list_norepet_NoDup :
+  forall (l : list A), list_norepet l -> NoDup l.
+Proof.
+  intros l H. induction H; constructor; assumption.
+Qed.
+
+Lemma norepet_incl_length :
+  forall (l m : list A),
+    list_norepet l ->
+    (forall w, In w l -> In w m) ->
+    length l <= length m.
+Proof.
+  intros l m Hnr Hincl.
+  apply NoDup_incl_length.
+  - apply list_norepet_NoDup. exact Hnr.
+  - intros w Hw. apply Hincl. exact Hw.
+Qed.
+
+Lemma has_duplicates_false_norepet :
+  forall l, has_duplicates Aeqb l = false -> list_norepet l.
+Proof.
+  intros l H.
+  apply (has_duplicates_correct A Aeqb Aeqb_refl Aeqb_sym).
+  exact H.
+Qed.
+
+(* ------------------------------------------------------------------ *)
+(* Main lemma                                                          *)
+(* ------------------------------------------------------------------ *)
+
+Lemma is_dag_prop_bool_lemma :
+  forall (g : graph) (nodes : list A),
+    (forall u v, g u v = true -> In u nodes /\ In v nodes) ->
+    (is_dag g <-> is_dagb g nodes = true).
+Proof.
+  intros g nodes Hedges. split.
+  - (* is_dag -> is_dagb *)
+    intros Hdag.
+    unfold is_dagb. apply forallb_forall.
+    intros x Hx.
+    apply negb_true_iff.
+    destruct (reachableb g nodes (length nodes) x x) eqn:Hr.
+    + (* contradiction: reachableb finds a self-walk *)
+      exfalso. apply (Hdag x).
+      apply (reachableb_sound g nodes (length nodes) x x Hr).
+    + reflexivity.
+  - (* is_dagb -> is_dag *)
+    intros Hdagb x [mid Hwalk].
+    (* shorten the walk to a no-duplicate one *)
+    destruct (shorten_walk_nodup g x x mid Hwalk)
+      as [mid' [Hwalk' [Hnodup _]]].
+    (* its intermediate vertices are in nodes *)
+    assert (Hin : forall w, In w mid' -> In w nodes).
+    { apply (walk_mid_in_nodes g nodes x mid' x Hedges Hwalk'). }
+    (* hence its length is <= |nodes| *)
+    assert (Hlen : length mid' <= length nodes).
+    { apply norepet_incl_length.
+      - apply has_duplicates_false_norepet. exact Hnodup.
+      - exact Hin. }
+    (* so reachableb finds it *)
+    assert (Hr : reachableb g nodes (length nodes) x x = true).
+    { apply (walk_reachableb g nodes mid' x x Hin Hwalk' Hlen). }
+    (* but is_dagb says it must be false *)
+    unfold is_dagb in Hdagb.
+    rewrite forallb_forall in Hdagb.
+    (* x is in nodes because the walk has at least one edge from x *)
+    assert (Hxin : In x nodes).
+    { (* first edge of the walk: g x (head of mid' ++ [x]) *)
+      destruct mid' as [|m ms].
+      - simpl in Hwalk'. destruct Hwalk' as [Hedge _].
+        apply (Hedges x x Hedge).
+      - simpl in Hwalk'. destruct Hwalk' as [Hedge _].
+        apply (Hedges x m Hedge). }
+    specialize (Hdagb x Hxin).
+    apply negb_true_iff in Hdagb.
+    rewrite Hr in Hdagb. discriminate.
+Qed.
+
+End PosGraph.
